code/ecdsap256/Hacl.Impl.Q.BasePointHiding.fst
@@ -1,0 +1,56 @@
+module Hacl.Impl.Q.BasePointHiding
+
+
+open FStar.HyperStack.All
+open FStar.HyperStack
+module ST = FStar.HyperStack.ST
+
+open Lib.IntTypes
+open Lib.Buffer
+
+open Hacl.Impl.P256.LowLevel
+
+open Spec.P256
+open Spec.P256.Definitions
+
+open FStar.Mul
+
+
+open Hacl.Impl.P256.LowLevel.PrimeSpecific
+open Lib.Loops
+
+open Lib.IntTypes.Intrinsics
+
+open Spec.P256.MontgomeryMultiplication
+open Hacl.Impl.P256.Core
+
+
+
+(* usually p -> toDomain -> ... -> fromDomain -> r *)
+
+val basePointRandomisation: p: point -> resultPoint: point -> 
+  Stack unit 
+    (requires fun h -> live h p /\ live h resultPoint)
+    (ensures fun h0 _ h1 -> 
+      let resultPoint = point_prime_to_coordinates (as_seq h1 resultPoint) in 
+      let resultFromDomain = fromDomainPoint resultPoint in 
+      let pointOriginal = point_prime_to_coordinates (as_seq h0 p) in 
+      let resultNormalized = _norm resultFromDomain in 
+      pointOriginal == resultNormalized)
+      
+(* or this, depends *)
+      
+(*
+val basePointRandomisation: p: point -> resultPoint: point -> 
+  Stack unit 
+    (requires fun h -> live h p /\ live h resultPoint)
+    (ensures fun h0 _ h1 -> 
+      let resultPoint = point_prime_to_coordinates (as_seq h1 resultPoint) in 
+      let pointOriginal = point_prime_to_coordinates (as_seq h0 p) in 
+      let resultNormalized = _norm resultPoint in 
+      pointOriginal == resultNormalized)
+*)
+
+
+let basePointRandomisation p result = 
+  admit()
